Rough draft of regular_spec

Assigned/Dyer.v
@@ -1392,7 +1392,14 @@ Module Make (Owner : DecidableTypeBoth) (Map : FMapInterface.WSfun Owner).
       Prop :=
       State.Transition.t s t /\ State.Ok.t s.
 
-    Add Parametric Morphism : (fun s : State.t => Coloring.new s.(State.colors) s.(State.labeling)) with signature
+    Definition to_coloring
+      (s : State.t) :
+      Coloring.t :=
+      Coloring.new
+        s.(State.colors)
+        s.(State.labeling).
+
+    Add Parametric Morphism : to_coloring with signature
       (Transition_Ok ++> Coloring.le) as coloring_morphism.
     Proof with State.Ok.Ok_tac.
       intros s t (Transition_s_t & Ok_s).
@@ -1416,13 +1423,13 @@ Module Make (Owner : DecidableTypeBoth) (Map : FMapInterface.WSfun Owner).
       relation State.t :=
       clos_refl_trans_1n _ State.Transition.t.
 
-    Add Parametric Morphism : State.Ok.t with signature
+(*     Add Parametric Morphism : State.Ok.t with signature
       Graph ++> impl as Graph_morphism.
     Proof.
       intros s t Graph_s_t Ok_s.
-      now induction Graph_s_t as [| s s' t Transition_s_s' Graph_s'_t IHs'_t];
+      now induction Graph_s_t as [s| s s' t Transition_s_s' Graph_s'_t IHs'_t];
         [| apply IHs'_t; rewrite <- Transition_s_s'].
-    Qed.
+    Qed. *)
 
     Lemma regular_body_spec :
       forall
@@ -1472,6 +1479,387 @@ Module Make (Owner : DecidableTypeBoth) (Map : FMapInterface.WSfun Owner).
         (coloring' & unused_colors' & H & Graph_s'_t).
       exists coloring', unused_colors'.
       now split; [| constructor 2 with (2 := Graph_s'_t); constructor].
+    Qed.
+
+    Module M := MSetWeakList.Make Owner.
+    Module Active := Active M.
+    Module M_Properties := MSetProperties.WPropertiesOn Owner M.
+
+    Definition Count_Ok
+      (s : State.t) :
+      Prop :=
+      s.(State.colors) =
+        Active.count s.(State.instructions) +
+        length s.(State.unused_colors).
+
+    Add Parametric Morphism : Count_Ok with signature
+      Transition_Ok ++> impl as Count_morphism.
+    Proof.
+      intros s t (Transition_s_t & Ok_s).
+      pose proof Ok_s.(State.Ok.instructions) as Ok_instructions.
+      unfold Count_Ok.
+      induction Transition_s_t as [
+          p₀ x₀ colors labeling|
+        p₀ x₀ colors labeling unused_color unused_colors|
+      p₀ x₀ colors labeling used_color unused_colors p₀_to_used_color];
+      intros Count_s;
+          cbv [State.colors State.instructions State.unused_colors] in *.
+          now rewrite Count_s, <- plus_Sn_m, Active.count_Up.
+        change (length (unused_color :: unused_colors)) with (S (length unused_colors)) in Count_s.
+        now rewrite Count_s, <- plus_Snm_nSm, Active.count_Up.
+      now rewrite Count_s, Active.count_Down, plus_Snm_nSm.
+    Qed.
+
+    Add Parametric Morphism : State.instructions with signature
+      State.Transition.t ++> Tail (A := Instruction.t) as instructions_morphism.
+    Proof.
+      intros s t Transition_s_t.
+      induction Transition_s_t as [
+          p₀ x₀ colors labeling|
+        p₀ x₀ colors labeling unused_color unused_colors|
+      p₀ x₀ colors labeling used_color unused_colors p₀_to_used_color];
+      constructor.
+    Qed.
+
+    Instance Transition_Graph_subrelation :
+      subrelation State.Transition.t Graph.
+    Proof.
+      intros s s' Transition_s_s'.
+      now apply clos_rt1n_step.
+    Qed.
+
+    Generalizable Variables A R f.
+
+    Instance Graph_morphism
+      `{PreOrder_R : @PreOrder A R}
+      `{Proper_f : Proper _ (State.Transition.t ++> R) f} :
+      Proper (Graph ++> R) f.
+    Proof.
+      intros s t Graph_s_t.
+      induction Graph_s_t as
+        [s|
+      s s' t Transition_s_s' Graph_s'_t IHs'_t].
+        reflexivity.
+      now transitivity (f s'); [rewrite Transition_s_s'|].
+    Qed.
+
+    Definition Graph_Ok
+      (s t : State.t) :
+      Prop :=
+      Graph s t /\ State.Ok.t s.
+
+    Instance Graph_Ok_morphism
+      `{PreOrder_R : @PreOrder A R}
+      `{Proper_f : Proper _ (Transition_Ok ++> R) f} :
+      Proper (Graph_Ok ++> R) f.
+    Proof.
+      intros s t (Graph_s_t & Ok_s).
+      induction Graph_s_t as
+        [s|
+      s s' t Transition_s_s' Graph_s'_t IHs'_t].
+        reflexivity.
+      transitivity (f s').
+        now apply Proper_f.
+      now apply IHs'_t; rewrite <- Transition_s_s'.
+    Qed.
+
+    Add Parametric Relation : Prop impl
+      reflexivity proved by impl_Reflexive
+      transitivity proved by impl_Transitive
+      as PreOrder_impl.
+
+    Lemma Graph_invariant :
+      forall
+        s t : State.t,
+        Graph s t ->
+        State.Ok.t s ->
+        Count_Ok s ->
+        t.(State.instructions) = [] ->
+        Skip.Forall
+          (fun skip : Instructions.t =>
+          Active.count skip <= State.colors t)
+          s.(State.instructions).
+    Proof.
+      intros s t Graph_s_t.
+      induction Graph_s_t as
+        [s|
+      s s' t Transition_s_s' Graph_s'_t IHs'_t]; intros Ok_s Count_s.
+        intros -> skip Skip_x_skip.
+        apply List.Skip.nil_inv in Skip_x_skip as ->.
+        auto with arith.
+      intros H skip.
+
+      specialize instructions_morphism with (1 := Transition_s_s') as Tail.
+      apply Tail.inv in Tail as (u₀ & H').
+      rewrite H'.
+      intros Skip_x_skip.
+      apply Skip.cons_inv in Skip_x_skip as
+        [?|
+      ?].
+        rewrite H0.
+        transitivity (s.(State.colors)).
+        rewrite Count_s.
+        rewrite H'.
+        apply le_plus_l.
+
+        enough (Coloring.le (to_coloring s) (to_coloring t)).
+          firstorder.
+        transitivity (to_coloring s').
+          now apply coloring_morphism; split.
+          assert (X : Transition_Ok s s') by
+            now split.
+          assert (Y : Graph_Ok s' t).
+            split.
+              assumption.
+            now rewrite <- Transition_s_s'.
+          now rewrite Y.
+        apply IHs'_t.
+          now rewrite <- Transition_s_s'.
+          assert (X : Transition_Ok s s').
+            now split.
+          now rewrite <- X.
+        assumption.
+        assumption.
+    Qed.
+
+    Lemma Graph_invariant' :
+      forall
+        s t : State.t,
+        Graph s t ->
+        State.Ok.t s ->
+        Count_Ok s ->
+        s.(State.colors) = t.(State.colors) \/
+        Skip.Exists
+          (fun skip : Instructions.t =>
+          Active.count skip = t.(State.colors))
+          s.(State.instructions).
+    Proof.
+      intros s t Graph_s_t.
+      induction Graph_s_t as
+        [s|
+      s s' t Transition_s_s' Graph_s'_t IHs'_t]; intros Ok_s Count_s.
+        now left.
+      specialize IHs'_t as [e| (skip & Skip_x₀_skip & e)].
+            now rewrite <- Transition_s_s'.
+          enough (Transition_Ok_s_s' : Transition_Ok s s') by
+            now rewrite <- Transition_Ok_s_s'.
+          now split.
+        enough (s_le_s' : s.(State.colors) <= s'.(State.colors)).
+          apply Nat.le_lteq in s_le_s' as
+            [s_lt_s'|
+          s_eq_s'];
+            [right|
+          left].
+            enough (s'.(State.unused_colors) = []).
+              exists s'.(State.instructions); split.
+                apply List.Skip.Tail_subrelation.
+                now apply instructions_morphism.
+              rewrite <- e; enough (Count_Ok s') as ->.
+                rewrite H.
+                simpl; auto with arith.
+              now apply Count_morphism with (2 := Count_s).
+            induction Transition_s_s' as [
+                p₀ x₀ colors labeling|
+              p₀ x₀ colors labeling unused_color unused_colors|
+            p₀ x₀ colors labeling used_color unused_colors p₀_to_used_color];
+            simpl in *.
+                reflexivity.
+              1, 2 :
+              contradict s_lt_s'; auto with arith.
+          now rewrite s_eq_s'.
+        enough (Coloring.le (to_coloring s) (to_coloring s')) by
+          firstorder.
+        now apply coloring_morphism.
+      right.
+      exists skip; split.
+        now rewrite Transition_s_s'.
+      assumption.
+    Qed.
+
+    Definition Proper
+      (labeling : Map.t nat)
+      (instructions : Instructions.t) :
+      Prop :=
+      forall
+      (owner owner' : Owner.t)
+      (color : nat),
+      Active owner instructions /\ Map.MapsTo owner color labeling ->
+      Active owner' instructions /\ Map.MapsTo owner' color labeling ->
+      Owner.eq owner owner'.
+
+      Lemma Graph_invariant'' :
+      forall
+        s t : State.t,
+        Graph s t ->
+        State.Ok.t s ->
+        t.(State.instructions) = [] ->
+        Skip.Forall
+          (Proper t.(State.labeling))
+          s.(State.instructions).
+    Proof.
+      intros s t Graph_s_t.
+      induction Graph_s_t as
+        [s|
+      s s' t Transition_s_s' Graph_s'_t IHs'_t]; intros Ok_s.
+        intros e skip Skip_x_skip.
+        rewrite e in Skip_x_skip.
+        apply List.Skip.nil_inv in Skip_x_skip as ->.
+        rewrite <- e.
+        pose  (Ok_s.(State.Ok.proper)).
+        assumption.
+      intros e.
+      intros skip Skip_x_skip owner owner' color
+        Active_MapsTo_owner_color Active_MapsTo_owner'_color.
+      assert (Tail_s_s' : Tail s.(State.instructions) s'.(State.instructions)).
+        now apply instructions_morphism.
+      apply Tail.inv in Tail_s_s' as (u₀ & e').
+      rewrite e' in Skip_x_skip.
+      apply List.Skip.cons_inv in Skip_x_skip as [e''|
+        Skip_x₀_skip].
+        pose (H := Ok_s.(State.Ok.proper)).
+        rewrite e'', <- e' in
+          Active_MapsTo_owner_color,
+          Active_MapsTo_owner'_color.
+        destruct
+          Active_MapsTo_owner_color as
+          (Active_owner_skip & owner_to_color),
+          Active_MapsTo_owner'_color as
+          (Active_owner'_skip & owner'_to_color).
+        apply (H owner owner' color).
+
+        split.
+            easy.
+          apply Ok_s.(State.Ok.active) in Active_owner_skip
+            as (color' & owner_to_color').
+          enough (color = color') as ->.
+            easy.
+          apply MapsTo_fun with (1 := owner_to_color).
+          enough (Coloring.le
+            (to_coloring s)
+            (to_coloring t)).
+            now apply H0.
+          transitivity (to_coloring s').
+            now apply coloring_morphism.
+          change (Graph s' t) in Graph_s'_t.
+          enough (Graph_Ok_s'_t : Graph_Ok s' t).
+            now rewrite Graph_Ok_s'_t.
+          split.
+            assumption.
+          now rewrite <- Transition_s_s'.
+
+          split.
+            easy.
+          apply Ok_s.(State.Ok.active) in Active_owner'_skip
+            as (color' & owner'_to_color').
+          enough (color = color') as ->.
+            easy.
+          apply MapsTo_fun with (1 := owner'_to_color).
+          enough (Coloring.le
+            (to_coloring s)
+            (to_coloring t)).
+            now apply H0.
+          transitivity (to_coloring s').
+            now apply coloring_morphism.
+          change (Graph s' t) in Graph_s'_t.
+          enough (Graph_Ok_s'_t : Graph_Ok s' t).
+            now rewrite Graph_Ok_s'_t.
+          split.
+            assumption.
+          now rewrite <- Transition_s_s'.
+      rewrite Transition_s_s' in Ok_s.
+      now apply (IHs'_t Ok_s e skip Skip_x₀_skip owner owner' color).
+    Qed.
+
+    Lemma start_Ok :
+      forall
+      instructions : Instructions.t,
+      Instructions.Ok instructions ->
+      Instructions.Closed instructions ->
+      State.Ok.t
+        {|
+          State.instructions := instructions;
+          State.colors := 0;
+          State.labeling := Map.empty nat;
+          State.unused_colors := [];
+        |}.
+    Proof.
+      intros instructions Ok_instructions Closed_instructions.
+      specialize Closed_impl_not_Active with (1 := Closed_instructions) as
+        not_Active.
+      constructor.
+                  assumption.
+                apply Coloring.Ok.empty.
+              simpl.
+              intros owner Ahead_owner_instructions.
+              now rewrite empty_in_iff.
+            intros owner Active_owner_instructions.
+            now contradict Active_owner_instructions.
+          intros color.
+          split.
+            contradiction.
+          intros (color_lt_0 & _).
+          contradict color_lt_0; auto with arith.
+        intros owner owner' color (Active_owner_instructions & _);
+        now contradict Active_owner_instructions.
+      constructor.
+    Qed.
+
+    Lemma regular_spec :
+      forall
+      instructions : Instructions.t,
+      Instructions.Ok instructions ->
+      Instructions.Closed instructions ->
+      exists
+      coloring : Coloring.t,
+      Regular.regular instructions = Some coloring /\
+      Coloring.Ok coloring /\
+      Skip.Forall
+        (Proper coloring.(Coloring.labeling))
+        instructions /\
+      Skip.Forall
+        (fun skip : Instructions.t =>
+        Active.count instructions <= coloring.(Coloring.colors))
+        instructions /\
+      Skip.Exists
+        (fun skip : Instructions.t =>
+        Active.count skip = coloring.(Coloring.colors))
+        instructions.
+    Proof with State.Ok.Ok_tac.
+      intros instructions Ok_instructions Closed_instructions.
+      specialize start_Ok with
+        (1 := Ok_instructions)
+        (2 := Closed_instructions) as Ok_s.
+      pose (s :=
+      {|
+        State.instructions := instructions;
+        State.colors := 0;
+        State.labeling := Map.empty nat;
+        State.unused_colors := []
+      |}).
+      assert (Count_s : Count_Ok s).
+        unfold Count_Ok.
+        simpl.
+        rewrite Active.count_closed; auto with arith.
+      specialize regular_body_spec with (1 := Ok_s) as
+        (coloring' & unused_colors' & e & Graph_s_t).
+      exists coloring'.
+      split_left.
+              now rewrite <- e.
+            rewrite Graph_s_t in Ok_s.
+            apply Ok_s.
+          now apply Graph_invariant'' with (1 := Graph_s_t).
+        intros skip Skip_instructions_skip.
+        now apply Graph_invariant with (1 := Graph_s_t).
+      specialize Graph_invariant' with
+        (1 := Graph_s_t)
+        (2 := Ok_s)
+        (3 := Count_s) as
+        [?| ?]; simpl in *.
+        exists instructions.
+        split.
+          reflexivity.
+        now rewrite Active.count_closed.
+      assumption.
     Qed.
   End Regular'.
 
